Defined SizedQueue and made a first approximation at a general efficient implementation. Implemented Binomial Heaps from Okasaki, but no proofs yet.

ADT/QueueSpec.v
@@ -2,7 +2,7 @@ Add Rec LoadPath "/home/zeimer/Code/Coq".
 
 Require Import RCCBase.
 
-(* TODO *) Module Type QueueSpec.
+(* TODO *) Module Type Queue.
 
 Parameter Queue : Type -> Type.
 
@@ -21,9 +21,6 @@ Parameter head :
 Parameter tail :
   forall {A : Type}, Queue A -> option (Queue A).
 
-Parameter size :
-  forall {A : Type}, Queue A -> nat.
-
 (* Properties of [isEmpty]. *)
 Parameter isEmpty_empty :
   forall A : Type, isEmpty (@empty A) = true.
@@ -34,7 +31,7 @@ Parameter isEmpty_snoc :
 
 Parameter isEmpty_head_true :
   forall (A : Type) (q : Queue A),
-    isEmpty q = true <-> head q = None.
+    isEmpty q = true (*TODO: <*)-> head q = None.
 
 Parameter isEmpty_head_false :
   forall (A : Type) (q : Queue A),
@@ -47,14 +44,6 @@ Parameter isEmpty_tail_false :
 Parameter isEmpty_tail_true :
   forall (A : Type) (q : Queue A),
     isEmpty q = true <-> tail q = None.
-
-Parameter isEmpty_size_true :
-  forall (A : Type) (q : Queue A),
-    isEmpty q = true <-> size q = 0.
-
-Parameter isEmpty_size_false :
-  forall (A : Type) (q : Queue A),
-    isEmpty q = false <-> size q <> 0.
 
 (* Properties of [head]. *)
 Parameter head_empty :
@@ -80,13 +69,18 @@ Parameter tail_singl :
   forall (A : Type) (x : A),
     tail (snoc x empty) = Some empty.
 
+Hint Rewrite isEmpty_empty isEmpty_snoc head_empty head_singl
+             tail_empty tail_singl : Queue.
+
+End Queue.
+
 (* [fmap] and its properties. *)
-Parameter fmap :
+(*Parameter fmap :
   forall {A B : Type}, (A -> B) -> Queue A -> Queue B.
 
 Parameter fmap_empty :
   forall (A B : Type) (f : A -> B),
-    fmap f (@empty A) = @empty B.
+    fmap f (@empty) = @empty B.
 
 Parameter fmap_isEmpty :
   forall (A B : Type) (f : A -> B) (q : Queue A),
@@ -110,9 +104,15 @@ Parameter fmap_tail :
 
 Parameter fmap_size :
   forall (A B : Type) (f : A -> B) (q : Queue A),
-    size (fmap f q) = size q.
+    size (fmap f q) = size q.*)
 
-(** Properties of [size]. *)
+Module Type SizedQueue (Q : Queue).
+
+Import Q.
+
+Parameter size :
+  forall {A : Type}, Queue A -> nat.
+
 Parameter size_empty :
   forall A : Type, size (@empty A) = 0.
 
@@ -124,4 +124,103 @@ Parameter size_tail :
   forall (A : Type) (q q' : Queue A),
     tail q = Some q' -> size q' = pred (size q).
 
-End QueueSpec.
+Parameter size_isEmpty_true :
+  forall (A : Type) (q : Queue A),
+    isEmpty q = true <-> size q = 0.
+
+Parameter size_isEmpty_false :
+  forall (A : Type) (q : Queue A),
+    isEmpty q = false <-> size q <> 0.
+
+End SizedQueue.
+
+Module ConstantSizedQueue_Queue (Q : Queue) : Queue.
+
+Definition Queue (A : Type) := (nat * Q.Queue A)%type.
+
+Definition empty {A : Type} : Queue A := (0, Q.empty).
+
+Definition isEmpty {A : Type} (q : Queue A) : bool :=
+  Q.isEmpty (snd q).
+
+Definition snoc {A : Type} (x : A) (q : Queue A) : Queue A :=
+  let '(n, q') := q in (S n, Q.snoc x q').
+
+Definition head {A : Type} (q : Queue A) : option A :=
+  Q.head (snd q).
+
+Definition tail {A : Type} (q : Queue A) : option (Queue A) :=
+  let '(n, q') := q in
+match Q.tail q' with
+    | None => None
+    | Some q'' => Some (pred n, q'')
+end.
+
+Ltac sized := repeat
+match goal with
+    | |- forall q : Queue _, _ => destruct q
+    | |- forall _, _ => intro
+end;
+  compute; autorewrite with Queue; try reflexivity.
+
+Lemma isEmpty_empty : forall A : Type, isEmpty (@empty A) = true.
+Proof. sized. Qed.
+
+Lemma isEmpty_snoc :
+  forall (A : Type) (x : A) (q : Queue A), isEmpty (snoc x q) = false.
+Proof. sized. Qed.
+
+Lemma isEmpty_head_true :
+  forall (A : Type) (q : Queue A), isEmpty q = true (*<*)-> head q = None.
+Proof. sized. Admitted.
+
+(*  Hint Resolve Q.isEmpty_head_true : wut.
+  Check Q.isEmpty_head_true. auto with wut. auto with wut.*)
+
+Lemma isEmpty_head_false :
+  forall (A : Type) (q : Queue A),
+    isEmpty q = false <-> exists h : A, head q = Some h.
+Proof. sized. Admitted.
+
+Lemma isEmpty_tail_false :
+  forall (A : Type) (q : Queue A),
+    isEmpty q = false <-> (exists q' : Queue A, tail q = Some q').
+Proof. sized. Admitted.
+
+Lemma isEmpty_tail_true :
+  forall (A : Type) (q : Queue A), isEmpty q = true <-> tail q = None.
+Proof. sized. Admitted.
+
+Lemma head_empty :
+  forall A : Type, head (@empty A) = None.
+Proof. sized. Qed.
+
+Lemma head_singl :
+  forall (A : Type) (x : A), head (snoc x empty) = Some x.
+Proof. sized. Qed.
+
+Lemma head_snoc_false :
+  forall (A : Type) (x : A) (q : Queue A),
+    isEmpty q = false -> head (snoc x q) = head q.
+Proof. sized. Admitted.
+
+Lemma head_snoc_true :
+  forall (A : Type) (x : A) (q : Queue A),
+    isEmpty q = true -> head (snoc x q) = Some x.
+Proof. sized. Admitted.
+
+Lemma tail_empty :
+  forall A : Type, tail (@empty A) = None.
+Proof. sized. Qed.
+
+Lemma tail_singl :
+  forall (A : Type) (x : A), tail (snoc x empty) = Some empty.
+Proof. sized. Qed.
+
+End ConstantSizedQueue_Queue.
+
+Module ConstantSizedQueue (Q : Queue)
+  : SizedQueue (ConstantSizedQueue_Queue Q).
+
+End ConstantSizedQueue.
+ ConstantSizedQueue_Queue.
