DS/BinomialHeap.v
@@ -1,0 +1,128 @@
+Add Rec LoadPath "/home/zeimer/Code/Coq".
+
+Require Export LinDec.
+Require Export RCCBase.
+
+Inductive Tree (A : Type) : Type :=
+    | T : nat -> A -> list (Tree A) -> Tree A.
+
+Arguments T [A] _ _ _.
+
+Definition Heap (A : Type) : Type := list (Tree A).
+
+Definition empty {A : Type} : Heap A := [].
+
+Definition isEmpty {A : Type} (h : Heap A) : bool :=
+match h with
+    | [] => true
+    | _ => false
+end.
+
+Definition rank {A : Type} (t : Tree A) : nat :=
+match t with
+    | T r _ _ => r
+end.
+
+Definition root {A : Type} (t : Tree A) : A :=
+match t with
+    | T _ x _ => x
+end.
+
+Function link {A : LinDec} (t1 t2 : Tree A) : Tree A :=
+match t1, t2 with
+    | T r x ts1, T _ y ts2 =>
+        if x <=? y
+        then T (S r) x (t2 :: ts1)
+        else T (S r) y (t1 :: ts2)
+end.
+
+Fixpoint insTree {A : LinDec} (t : Tree A) (h : Heap A) : Heap A :=
+match h with
+    | [] => [t]
+    | t' :: h' =>
+        if rank t <? rank t'
+        then t :: h
+        else insTree (link t t') h'
+end.
+
+Definition insert {A : LinDec} (x : A) (h : Heap A) : Heap A :=
+  insTree (T 0 x []) h.
+
+Fixpoint merge {A : LinDec} (h1 h2 : Heap A) : Heap A :=
+match h1 with
+    | [] => h2
+    | t1 :: h1' =>
+        let
+          aux := fix aux (h2 : Heap A) : Heap A :=
+          match h2 with
+              | [] => h1
+              | t2 :: h2' =>
+                  if rank t1 <? rank t2
+                  then t1 :: merge h1' h2
+                  else
+                    if rank t2 <? rank t1
+                    then t2 :: aux h2'
+                    else insTree (link t1 t2) (merge h1' h2')
+          end
+        in aux h2
+end.
+
+(*Fixpoint merge {A : LinDec} (h1 h2 : Heap A) : Heap A :=
+match h1, h2 with
+    | [], _ => h2
+    | _, [] => h1
+    | t1 :: h1', t2 :: h2' =>
+        if rank t1 <? rank t2
+        then t1 :: merge h1' h2
+        else
+          if rank t2 <? rank t1
+          then t2 :: merge h1 h2'
+          else insTree (link t1 t2) (merge h1' h2')
+end.*)
+
+Lemma merge_spec :
+  forall (A : LinDec) (h1 h2 : Heap A),
+    merge h1 h2 =
+    match h1, h2 with
+        | [], _ => h2
+        | _, [] => h1
+        | t1 :: h1', t2 :: h2' =>
+            if rank t1 <? rank t2
+            then t1 :: merge h1' h2
+            else
+              if rank t2 <? rank t1
+              then t2 :: merge h1 h2'
+              else insTree (link t1 t2) (merge h1' h2')
+    end.
+Proof.
+  destruct h1, h2; reflexivity.
+Qed.
+
+Fixpoint removeMinTree
+  {A : LinDec} (h : Heap A) : option (Tree A * Heap A) :=
+match h with
+    | [] => None
+    | [t] => Some (t, [])
+    | t :: h' =>
+        match removeMinTree h' with
+            | None => None
+            | Some (t', h'') =>
+                if (root t <=? root t') && negb (root t =? root t')
+                then Some (t, h')
+                else Some (t', t :: h'')
+        end
+end.
+
+Definition findMin {A : LinDec} (h : Heap A) : option A :=
+match removeMinTree h with
+    | None => None
+    | Some (t, _) => Some (root t)
+end.
+
+Definition deleteMin {A : LinDec} (h : Heap A) : option (Heap A) :=
+match removeMinTree h with
+    | None => None
+    | Some (T _ x h1, h2) => Some (merge h1 h2)
+end.
+
+Import PriorityQueue.
